Modified semantics for more rigorous transaction conditions

src/Prototype/Transaction.v
@@ -3,65 +3,89 @@ Require Import FnMap Language.
 
 Section System.
   Context {MsgT StateT: Type}.
+  Context {MvalT: MsgT -> RqRs -> Type}.
+  Hypothesis (msgT_dec : forall m1 m2 : MsgT, {m1 = m2} + {m1 <> m2}).
+
+  Local Notation isTrsPair := (isTrsPair msgT_dec).
 
   Definition CondT := StateT -> Prop.
   Definition condImp (c1 c2: CondT) := forall st, c1 st -> c2 st.
   Infix "-->" := condImp (at level 30).
-  Definition postOf (postcond: StateT -> MsgT -> StateT -> Prop): CondT :=
-    fun post => forall pre mt, postcond pre mt post.
+  Definition postOf (pmsg: PMsg MvalT StateT): CondT :=
+    fun post => forall pre mt, pmsg_postcond pmsg pre mt post.
 
   Definition Disjoint (c1 c2: CondT) := forall st, c1 st -> c2 st -> False.
   Infix "-*-" := Disjoint (at level 30).
 
   Section PerObject.
-    Variable obj: Object MsgT StateT.
+    Variable obj: Object MvalT StateT.
 
-    Definition Transaction (rq rsr: PMsg MsgT StateT) (rs: Msg MsgT) :=
-      In rq (obj_pmsgs obj) /\ In rsr (obj_pmsgs obj) /\
-      (exists st mt, In rs (outsOf rsr st mt)) /\
-      isTrsPair (midOf rq) (msg_id rs) = true.
+    (*! Transaction *)
 
     (* A VERY SUBTLE POINT:
      * [rsr] is not a [PMsg] that handles the response,
      * but a [PMsg] that _sends_ the response.
      *)
-    Inductive TransactionInv: PMsg MsgT StateT (* request *) ->
+    Definition Transaction (rq rsr: PMsg MvalT StateT) (rs: Msg MvalT) :=
+      In rq (obj_pmsgs obj) /\ In rsr (obj_pmsgs obj) /\
+      (exists st mt, In rs (pmsg_outs rsr st mt)) /\
+      isTrsPair (pmsg_mid rq) (msg_id rs) = true.
+
+    Inductive TransactionInv: PMsg MvalT StateT (* request *) ->
                               CondT ->
-                              PMsg MsgT StateT (* response *) -> Prop :=
+                              PMsg MvalT StateT (* response *) -> Prop :=
     | TrsInv: forall rq rsr trsinv,
-        postOf (postcondOf rq) --> trsinv ->
-        trsinv --> precondOf rsr ->
-        (forall pmsg, In pmsg (obj_pmsgs obj) ->
-                      pmsg <> rsr ->
-                      (precondOf pmsg) -*- trsinv) ->
+        postOf rq --> trsinv ->
+        trsinv --> pmsg_precond rsr ->
         TransactionInv rq trsinv rsr.
+
+    (*! LocallyDisjoint *)
+
+    Definition DisjointTrsInv (rsr: PMsg MvalT StateT) (trsinv: CondT) :=
+      forall pmsg, In pmsg (obj_pmsgs obj) ->
+                   pmsg <> rsr ->
+                   (pmsg_precond pmsg) -*- trsinv.
 
     Definition LocallyDisjoint :=
       forall rq rsr rs,
         Transaction rq rsr rs ->
         exists trsinv,
-          TransactionInv rq trsinv rsr.
+          TransactionInv rq trsinv rsr /\
+          DisjointTrsInv rsr trsinv.
 
-    Definition Immediate (rq: PMsg MsgT StateT) :=
-      msg_rqrs (midOf rq) = Rq /\
+    (*! Restricted interference *)
+
+    (* Interferences are allowed only by prioritizers. Specifically, during a 
+     * given transaction handling a request from a process (object) with index "i":
+     * 1) Any other transactions with indices >= i should be disjoint.
+     * 2) Transactions with indices < i are allowed to interleave, but they should
+     *    be locally linearizable.
+     *)
+
+    (* TODO: formalize *)
+
+    (*! Monotonicity *)
+    
+    Definition Immediate (rq: PMsg MvalT StateT) :=
+      msg_rqrs (pmsg_mid rq) = Rq /\
       forall st mt, exists rs,
-          outsOf rq st mt = rs :: nil /\
-          isTrsPair (midOf rq) (msg_id rs) = true.
+          pmsg_outs rq st mt = rs :: nil /\
+          isTrsPair (pmsg_mid rq) (msg_id rs) = true.
 
-    Definition Forwarding (rq1 rs2: PMsg MsgT StateT) :=
-      msg_rqrs (midOf rq1) = Rq /\
-      msg_rqrs (midOf rs2) = Rs /\
+    Definition Forwarding (rq1 rs2: PMsg MvalT StateT) :=
+      msg_rqrs (pmsg_mid rq1) = Rq /\
+      msg_rqrs (pmsg_mid rs2) = Rs /\
       (forall st mt, exists rq2,
-            outsOf rq1 st mt = rq2 :: nil /\
-            isTrsPair (msg_id rq2) (midOf rs2) = true) /\
+            pmsg_outs rq1 st mt = rq2 :: nil /\
+            isTrsPair (msg_id rq2) (pmsg_mid rs2) = true) /\
       (forall st mt, exists rs1,
-            outsOf rs2 st mt = rs1 :: nil /\
-            isTrsPair (midOf rq1) (msg_id rs1) = true).
+            pmsg_outs rs2 st mt = rs1 :: nil /\
+            isTrsPair (pmsg_mid rq1) (msg_id rs1) = true).
 
-    Definition UniqueHandler (pmsgs: list (PMsg MsgT StateT))
-               (pmsg: PMsg MsgT StateT) :=
+    Definition UniqueHandler (pmsgs: list (PMsg MvalT StateT))
+               (pmsg: PMsg MvalT StateT) :=
       In pmsg pmsgs /\
-      forall pmsg', In pmsg' pmsgs -> midOf pmsg <> midOf pmsg'.
+      forall pmsg', In pmsg' pmsgs -> (pmsg_mid pmsg) <> (pmsg_mid pmsg').
     
     (* Monotonicity is one of key factors whether a given protocol in a 
      * message-passing system is linearizable or not. It basically requires the
@@ -69,33 +93,35 @@ Section System.
      * object is monotone if there is no predicated message that
      * receives a response and sends some requests.
      *)
-    Definition MonotonePMsgs (pmsgs: list (PMsg MsgT StateT)): Prop :=
-      forall pmsg,
+    Definition MonotonePMsgs (pmsgs: list (PMsg MvalT StateT)): Prop :=
+      forall (pmsg: PMsg MvalT StateT),
         In pmsg pmsgs ->
         (Immediate pmsg \/
-         (exists rs, Forwarding pmsg rs /\ UniqueHandler pmsgs rs) \/
-         (exists rq, Forwarding rq pmsg /\ UniqueHandler pmsgs pmsg)).
+         (exists (rs: PMsg MvalT StateT),
+             Forwarding pmsg rs /\ UniqueHandler pmsgs rs) \/
+         (exists (rq: PMsg MvalT StateT),
+             Forwarding rq pmsg /\ UniqueHandler pmsgs pmsg)).
 
     Definition Monotone := MonotonePMsgs (obj_pmsgs obj).
 
   End PerObject.
 
   Section PerSystem.
-    Variable sys: System MsgT StateT.
+    Variable sys: System MvalT StateT.
 
-    Theorem sequential_linear: SequentialSys sys -> Linear sys.
+    Theorem sequential_linear: SequentialSys msgT_dec sys -> Linear msgT_dec sys.
     Proof.
     Admitted.
     
   End PerSystem.
 
   Theorem locally_disjoint_sequential:
-    forall obj, LocallyDisjoint obj -> SequentialSys (obj :: nil).
+    forall obj, LocallyDisjoint obj -> SequentialSys msgT_dec (obj :: nil).
   Proof.
   Admitted.
 
   Corollary locally_disjoint_linear:
-    forall obj, LocallyDisjoint obj -> Linear (obj :: nil).
+    forall obj, LocallyDisjoint obj -> Linear msgT_dec (obj :: nil).
   Proof.
     intros; apply sequential_linear, locally_disjoint_sequential; auto.
   Qed.
@@ -103,23 +129,26 @@ Section System.
 End System.
 
 Section Compositional.
+  Context {MsgT StateT: Type}.
+  Context {MvalT: MsgT -> RqRs -> Type}.
+  Hypothesis (msgT_dec : forall m1 m2 : MsgT, {m1 = m2} + {m1 <> m2}).
 
   Theorem linear_sequential_compositional:
-    forall {MsgT StateT} (sys: System MsgT StateT),
-      Forall Monotone sys ->
-      Forall (fun obj => SequentialSys (obj :: nil)) sys ->
-      Linear sys.
+    forall (sys: System MvalT StateT),
+      Forall (Monotone msgT_dec) sys ->
+      Forall (fun obj => SequentialSys msgT_dec (obj :: nil)) sys ->
+      Linear msgT_dec sys.
   Proof.
   Admitted.
 
   Corollary disjoint_linear:
-    forall {MsgT StateT} (sys: System MsgT StateT),
-      Forall Monotone sys ->
-      Forall LocallyDisjoint sys ->
-      Linear sys.
+    forall (sys: System MvalT StateT),
+      Forall (Monotone msgT_dec) sys ->
+      Forall (LocallyDisjoint msgT_dec) sys ->
+      Linear msgT_dec sys.
   Proof.
     intros; apply linear_sequential_compositional; auto.
-    apply Forall_impl with (P:= LocallyDisjoint); auto.
+    apply Forall_impl with (P:= LocallyDisjoint msgT_dec); auto.
     intros; apply locally_disjoint_sequential; auto.
   Qed.
 
