src/Prototype/SingleValue.v
@@ -5,15 +5,23 @@ Set Implicit Arguments.
 
 Open Scope list.
 
-Inductive SingleValueMsg : Set :=
-(* external *)
-| GetReq : SingleValueMsg
-| GetResp (v: nat) : SingleValueMsg
-| SetReq (v: nat) : SingleValueMsg
-| SetResp : SingleValueMsg
-(* internal *)
-| InvReq : SingleValueMsg
-| InvResp (v: nat) : SingleValueMsg.
+Inductive SingleValueMsgType :=
+| SvmGet
+| SvmSet
+| SvmInv.
+
+Definition svm_dec: forall m1 m2: SingleValueMsgType, {m1 = m2} + {m1 <> m2}.
+Proof.
+  decide equality.
+Defined.
+
+Inductive SingleValueMsg : SingleValueMsgType -> RqRs -> Set :=
+| GetReq : SingleValueMsg SvmGet Rq
+| GetResp (v: nat) : SingleValueMsg SvmGet Rs
+| SetReq (v: nat) : SingleValueMsg SvmSet Rq
+| SetResp : SingleValueMsg SvmSet Rs
+| InvReq : SingleValueMsg SvmInv Rq
+| InvResp (v: nat) : SingleValueMsg SvmInv Rs.
 
 Notation "'T'" := (fun _ => True).
 Notation "'TT'" := (fun pre _ post => pre = post).
@@ -29,19 +37,29 @@ Section System.
     Section PerExt.
       Variable extIdx: nat.
 
-      Definition getReqM := buildMsgId extIdx specIdx Rq.
-      Definition getRespM := buildMsgId extIdx specIdx Rs.
-      Definition setReqM := buildMsgId extIdx specIdx Rq.
-      Definition setRespM := buildMsgId extIdx specIdx Rs.
+      Definition getReqM := buildMsgId extIdx specIdx SvmGet Rq.
+      Definition getRespM := buildMsgId extIdx specIdx SvmGet Rs.
+      Definition setReqM := buildMsgId extIdx specIdx SvmSet Rq.
+      Definition setRespM := buildMsgId extIdx specIdx SvmSet Rs.
 
       Definition specGetReq: PMsg SingleValueMsg SpecState :=
-        Pmsg getReqM T
-             (fun st _ => {| msg_id := getRespM; msg_content := GetResp st |} :: nil)
-             (fun pre msg post => pre = post).
+        {| pmsg_mid := getReqM;
+           pmsg_precond := T;
+           pmsg_outs :=
+             fun st _ => {| msg_id := getRespM; msg_value := GetResp st |} :: nil;
+           pmsg_postcond :=
+             fun pre msg post => pre = post
+        |}.
+
       Definition specSetReq: PMsg SingleValueMsg SpecState :=
-        Pmsg setReqM T
-             (fun st _ => {| msg_id := setRespM; msg_content := SetResp |} :: nil)
-             (fun pre msg post => exists v, msg = SetReq v /\ post = v).
+        {| pmsg_mid := setReqM;
+           pmsg_precond := T;
+           pmsg_outs :=
+             fun st _ => {| msg_id := setRespM; msg_value := SetResp |} :: nil;
+           pmsg_postcond :=
+             fun pre (msg : SingleValueMsg (msg_type setReqM) (msg_rqrs setReqM)) post =>
+               exists v : nat, msg = SetReq v /\ post = v
+        |}.
 
     End PerExt.
 
@@ -85,79 +103,109 @@ Section System.
     Section Child.
       Variable childIdx: nat.
 
-      Definition ecGetReqM := buildMsgId (getExtIdx childIdx) childIdx Rq.
-      Definition ecGetRespM := buildMsgId (getExtIdx childIdx) childIdx Rs.
-      Definition ecSetReqM := buildMsgId (getExtIdx childIdx) childIdx Rq.
-      Definition ecSetRespM := buildMsgId (getExtIdx childIdx) childIdx Rs.
-      Definition cpGetReqM := buildMsgId childIdx parentIdx Rq.
-      Definition cpGetRespM := buildMsgId childIdx parentIdx Rs.
-      Definition cpSetReqM := buildMsgId childIdx parentIdx Rq.
-      Definition cpSetRespM := buildMsgId childIdx parentIdx Rs.
-      Definition pcInvReqM := buildMsgId parentIdx childIdx Rq.
-      Definition pcInvRespM := buildMsgId parentIdx childIdx Rs.
+      Definition ecGetReqM := buildMsgId (getExtIdx childIdx) childIdx SvmGet Rq.
+      Definition ecGetRespM := buildMsgId (getExtIdx childIdx) childIdx SvmGet Rs.
+      Definition ecSetReqM := buildMsgId (getExtIdx childIdx) childIdx SvmSet Rq.
+      Definition ecSetRespM := buildMsgId (getExtIdx childIdx) childIdx SvmSet Rs.
+      Definition cpGetReqM := buildMsgId childIdx parentIdx SvmGet Rq.
+      Definition cpGetRespM := buildMsgId childIdx parentIdx SvmGet Rs.
+      Definition cpSetReqM := buildMsgId childIdx parentIdx SvmSet Rq.
+      Definition cpSetRespM := buildMsgId childIdx parentIdx SvmSet Rs.
+      Definition pcInvReqM := buildMsgId parentIdx childIdx SvmInv Rq.
+      Definition pcInvRespM := buildMsgId parentIdx childIdx SvmInv Rs.
 
       Definition ecGetReqValid: PMsg SingleValueMsg ImplState :=
-        Pmsg ecGetReqM
-             (fun st => impl_status st = Valid)
-             (fun st _ => {| msg_id := ecGetRespM;
-                             msg_content := GetResp (impl_value st) |} :: nil)
-             (fun pre msg post => msg = GetReq /\ pre = post).
+        {| pmsg_mid := ecGetReqM;
+           pmsg_precond := fun st => impl_status st = Valid;
+           pmsg_outs :=
+             fun st _ => {| msg_id := ecGetRespM;
+                            msg_value := GetResp (impl_value st) |} :: nil;
+           pmsg_postcond :=
+             fun pre (msg: SingleValueMsg (msg_type ecGetReqM) (msg_rqrs ecGetReqM)) post =>
+               msg = GetReq /\ pre = post
+        |}.
       
       Definition ecGetReqInvalid: PMsg SingleValueMsg ImplState :=
-        Pmsg ecGetReqM
-             (fun st => impl_status st = Invalid)
-             (fun st _ => {| msg_id := cpGetReqM;
-                             msg_content := GetReq |} :: nil)
-             (fun pre msg post => msg = GetReq /\ impl_status post = Transient).
+        {| pmsg_mid := ecGetReqM;
+           pmsg_precond := fun st => impl_status st = Invalid;
+           pmsg_outs :=
+             fun st _ => {| msg_id := cpGetReqM;
+                            msg_value := GetReq |} :: nil;
+           pmsg_postcond :=
+             fun pre (msg: SingleValueMsg (msg_type ecGetReqM) (msg_rqrs ecGetReqM)) post =>
+               msg = GetReq /\ impl_status post = Transient
+      |}.
 
       Definition ecSetReqValid: PMsg SingleValueMsg ImplState :=
-        Pmsg ecSetReqM
-             (fun st => impl_status st = Valid)
-             (fun st _ => {| msg_id := ecSetRespM;
-                             msg_content := SetResp |} :: nil)
-             (fun pre msg post => exists v, msg = SetReq v /\
-                                            impl_status post = Valid /\
-                                            impl_value post = v).
+        {| pmsg_mid := ecSetReqM;
+           pmsg_precond := fun st => impl_status st = Valid;
+           pmsg_outs :=
+             fun st _ => {| msg_id := ecSetRespM;
+                            msg_value := SetResp |} :: nil;
+           pmsg_postcond :=
+             fun pre (msg: SingleValueMsg (msg_type ecSetReqM) (msg_rqrs ecSetReqM)) post =>
+               exists v, msg = SetReq v /\
+                         impl_status post = Valid /\
+                         impl_value post = v
+        |}.
 
       Definition ecSetReqInvalid: PMsg SingleValueMsg ImplState :=
-        Pmsg ecSetReqM
-             (fun st => impl_status st = Invalid)
-             (fun st msg =>
-                match msg with
-                | SetReq v => {| msg_id := cpSetReqM;
-                                 msg_content := SetReq v |} :: nil
-                | _ => nil
-                end)
-             (fun pre msg post => exists v, msg = SetReq v /\
-                                            impl_status post = Transient /\
-                                            impl_value_trs post = v).
+        {| pmsg_mid := ecSetReqM;
+           pmsg_precond := fun st => impl_status st = Invalid;
+           pmsg_outs :=
+             fun st msg =>
+               match msg with
+               | SetReq v => {| msg_id := cpSetReqM;
+                                msg_value := SetReq v |} :: nil
+               | _ => nil
+               end;
+           pmsg_postcond :=
+             fun pre (msg: SingleValueMsg (msg_type ecSetReqM) (msg_rqrs ecSetReqM)) post =>
+               exists v, msg = SetReq v /\
+                         impl_status post = Transient /\
+                         impl_value_trs post = v
+        |}.
 
       Definition cpGetResp: PMsg SingleValueMsg ImplState :=
-        Pmsg cpGetRespM T
-             (fun st msg =>
-                match msg with
-                | GetResp v => {| msg_id := ecGetRespM;
-                                  msg_content := GetResp v |} :: nil
-                | _ => nil
-                end)
-             (fun pre msg post => exists v, msg = GetResp v /\
-                                            impl_status post = Valid /\
-                                            impl_value post = v).
+        {| pmsg_mid := cpGetRespM;
+           pmsg_precond := T;
+           pmsg_outs :=
+             fun st msg =>
+               match msg with
+               | GetResp v => {| msg_id := ecGetRespM;
+                                 msg_value := GetResp v |} :: nil
+               | _ => nil
+               end;
+           pmsg_postcond :=
+             fun pre (msg: SingleValueMsg (msg_type cpGetRespM) (msg_rqrs cpGetRespM)) post =>
+               exists v, msg = GetResp v /\
+                         impl_status post = Valid /\
+                         impl_value post = v
+        |}.
 
       Definition cpSetResp: PMsg SingleValueMsg ImplState :=
-        Pmsg cpSetRespM T
-             (fun st _ => {| msg_id := ecSetRespM;
-                             msg_content := SetResp |} :: nil)
-             (fun pre msg post => msg = SetResp /\
-                                  impl_status post = Valid /\
-                                  impl_value post = impl_value_trs pre).
+        {| pmsg_mid := cpSetRespM;
+           pmsg_precond := T;
+           pmsg_outs :=
+             fun st _ => {| msg_id := ecSetRespM;
+                            msg_value := SetResp |} :: nil;
+           pmsg_postcond :=
+             fun pre (msg: SingleValueMsg (msg_type cpSetRespM) (msg_rqrs cpSetRespM)) post =>
+               msg = SetResp /\
+               impl_status post = Valid /\
+               impl_value post = impl_value_trs pre
+        |}.
 
       Definition pcInvReq: PMsg SingleValueMsg ImplState :=
-        Pmsg pcInvReqM
-             (fun st => impl_status st = Valid)
-             (fun st _ => {| msg_id := pcInvRespM;
-                             msg_content := InvResp (impl_value st) |} :: nil)
-             (fun pre msg post => msg = InvReq /\ impl_status post = Invalid).
+        {| pmsg_mid := pcInvReqM;
+           pmsg_precond := fun st => impl_status st = Valid;
+           pmsg_outs :=
+             fun st _ => {| msg_id := pcInvRespM;
+                            msg_value := InvResp (impl_value st) |} :: nil;
+           pmsg_postcond :=
+             fun pre (msg: SingleValueMsg (msg_type pcInvReqM) (msg_rqrs pcInvReqM)) post =>
+               msg = InvReq /\ impl_status post = Invalid
+        |}.
 
       Definition child: Object SingleValueMsg ImplState :=
         {| obj_idx := childIdx;
@@ -178,52 +226,84 @@ Section System.
     Section Parent.
 
       Definition cpGetReqValid childIdx: PMsg SingleValueMsg ImplState :=
-        Pmsg (cpGetReqM childIdx)
-             (fun st => impl_status st = Valid)
-             (fun st _ => {| msg_id := cpGetRespM childIdx;
-                             msg_content := GetResp (impl_value st) |} :: nil)
-             (fun pre msg post => msg = GetReq /\ impl_status post = Invalid).
+        {| pmsg_mid := cpGetReqM childIdx;
+           pmsg_precond := fun st => impl_status st = Valid;
+           pmsg_outs :=
+             fun st _ => {| msg_id := cpGetRespM childIdx;
+                            msg_value := GetResp (impl_value st) |} :: nil;
+           pmsg_postcond :=
+             fun pre (msg: SingleValueMsg (msg_type (cpGetReqM childIdx))
+                                          (msg_rqrs (cpGetReqM childIdx))) post =>
+               msg = GetReq /\ impl_status post = Invalid
+        |}.
       
       Definition cpGetReqInvalid childIdx: PMsg SingleValueMsg ImplState :=
-        Pmsg (cpGetReqM childIdx)
-             (fun st => impl_status st = Invalid)
-             (fun st _ => {| msg_id := pcInvReqM childIdx;
-                             msg_content := InvReq |} :: nil)
-             (fun pre msg post => msg = GetReq /\ impl_status post = Transient).
+        {| pmsg_mid := cpGetReqM childIdx;
+           pmsg_precond := fun st => impl_status st = Invalid;
+           pmsg_outs :=
+             fun st _ => {| msg_id := pcInvReqM childIdx;
+                            msg_value := InvReq |} :: nil;
+           pmsg_postcond :=
+             fun pre (msg: SingleValueMsg (msg_type (cpGetReqM childIdx))
+                                          (msg_rqrs (cpGetReqM childIdx))) post =>
+               msg = GetReq /\ impl_status post = Transient
+        |}.
 
       Definition cpSetReqValid childIdx: PMsg SingleValueMsg ImplState :=
-        Pmsg (cpSetReqM childIdx)
-             (fun st => impl_status st = Valid)
-             (fun st _ => {| msg_id := cpSetRespM childIdx;
-                             msg_content := SetResp |} :: nil)
-             (fun pre msg post => exists v, msg = SetReq v /\
-                                            impl_status post = Invalid).
+        {| pmsg_mid := cpSetReqM childIdx;
+           pmsg_precond := fun st => impl_status st = Valid;
+           pmsg_outs :=
+             fun st _ => {| msg_id := cpSetRespM childIdx;
+                            msg_value := SetResp |} :: nil;
+           pmsg_postcond :=
+             fun pre (msg: SingleValueMsg (msg_type (cpSetReqM childIdx))
+                                          (msg_rqrs (cpSetReqM childIdx))) post =>
+               exists v, msg = SetReq v /\
+                         impl_status post = Invalid
+        |}.
+      
       Definition cpSetReqInvalid childIdx: PMsg SingleValueMsg ImplState :=
-        Pmsg (cpSetReqM childIdx)
-             (fun st => impl_status st = Invalid)
-             (fun st _ => {| msg_id := pcInvReqM childIdx;
-                             msg_content := InvReq |} :: nil)
-             (fun pre msg post => exists v, msg = SetReq v /\
-                                            impl_status post = Transient).
+        {| pmsg_mid := cpSetReqM childIdx;
+           pmsg_precond := fun st => impl_status st = Invalid;
+           pmsg_outs :=
+             fun st _ => {| msg_id := pcInvReqM childIdx;
+                            msg_value := InvReq |} :: nil;
+           pmsg_postcond :=
+             fun pre (msg: SingleValueMsg (msg_type (cpSetReqM childIdx))
+                                          (msg_rqrs (cpSetReqM childIdx))) post =>
+               exists v, msg = SetReq v /\
+                         impl_status post = Transient
+        |}.
 
       Definition pcInvRespGet childIdx: PMsg SingleValueMsg ImplState :=
-        Pmsg (pcInvRespM childIdx)
-             (fun st => impl_status st = GetWait)
-             (fun st msg =>
-                match msg with
-                | InvResp v => {| msg_id := cpGetRespM childIdx;
-                                  msg_content := GetResp v |} :: nil
-                | _ => nil
-                end)
-             (fun pre msg post => exists v, msg = InvResp v /\
-                                            impl_status post = Invalid).
+        {| pmsg_mid := pcInvRespM childIdx;
+           pmsg_precond := fun st => impl_status st = GetWait;
+           pmsg_outs :=
+             fun st msg =>
+               match msg with
+               | InvResp v => {| msg_id := cpGetRespM childIdx;
+                                 msg_value := GetResp v |} :: nil
+               | _ => nil
+               end;
+           pmsg_postcond :=
+             fun pre (msg: SingleValueMsg (msg_type (pcInvRespM childIdx))
+                                          (msg_rqrs (pcInvRespM childIdx))) post =>
+               exists v, msg = InvResp v /\
+                         impl_status post = Invalid
+        |}.
+      
       Definition pcInvRespSet childIdx: PMsg SingleValueMsg ImplState :=
-        Pmsg (pcInvRespM childIdx)
-             (fun st => impl_status st = SetWait)
-             (fun st _ => {| msg_id := cpSetRespM childIdx;
-                             msg_content := SetResp |} :: nil)
-             (fun pre msg post => exists v, msg = InvResp v /\
-                                            impl_status post = Invalid).
+        {| pmsg_mid := pcInvRespM childIdx;
+           pmsg_precond := fun st => impl_status st = SetWait;
+           pmsg_outs :=
+             fun st _ => {| msg_id := cpSetRespM childIdx;
+                            msg_value := SetResp |} :: nil;
+           pmsg_postcond :=
+             fun pre (msg: SingleValueMsg (msg_type (pcInvRespM childIdx))
+                                          (msg_rqrs (pcInvRespM childIdx))) post =>
+               exists v, msg = InvResp v /\
+                         impl_status post = Invalid
+        |}.
 
       Definition parent : Object SingleValueMsg ImplState :=
         {| obj_idx := parentIdx;
